io/Compiler.Examples.fst
@@ -27,108 +27,138 @@ open Compiler.Model
   2b. HO
 **)
 
+(** Utils **)
+type source_arrow (arg:Type u#a) (res:Type u#b) (pre:arg -> trace -> Type0) (post:arg -> trace -> resexn res -> trace -> Type0) (fl:erased tflag) =
+  x:arg -> IIO (resexn res) fl (pre x) (post x)
+
+type c1typ (#arg:Type u#a) (#res:Type u#b) (pre:arg -> trace -> Type0) (post:arg -> trace -> resexn res -> trace -> Type0) (pi:monitorable_prop) =
+  squash (forall x h lt. pre x h /\ enforced_locally pi h lt ==> post x h (Inr Contract_failure) lt)
+  
+type c2typ (#arg:Type u#a) (#res:Type u#b) (pre:arg -> trace -> Type0) (post:arg -> trace -> resexn res -> trace -> Type0) (pi:monitorable_prop) (rc:rc_typ arg (resexn res)) =
+  squash (forall x h lt r. pre x h /\ enforced_locally pi h lt /\ rc x h r lt ==> post x h r lt)
+
+type stronger_pis (pi1:monitorable_prop) (pi2:monitorable_prop) =
+  squash (forall h lt. enforced_locally pi1 h lt ==> enforced_locally pi2 h lt)
+
 
 (** ** Testing **)
-(** *** Example 1 - FO **)
-let ex1_ct_pre = (fun () h -> True)
-let ex1_ct_post = (fun () h (rfd:resexn file_descr) lt -> (forall fd'. ~((EOpenfile "/etc/passwd" fd') `List.memP` lt)) /\ (Inl? rfd ==> is_open (Inl?.v rfd) (rev lt @ h)))
-let ex1_spec_pi : monitorable_prop = (fun cmd arg h -> match cmd, arg with | Openfile, s -> if s = "/etc/passwd" then false else true | _ -> true)
-let ex1_inst_pi : monitorable_prop = ex1_spec_pi
-let ex1_ct_rc = (fun () h (rfd:resexn file_descr) lt -> Inl? rfd && (is_open (Inl?.v rfd) (rev lt @ h)))
+(** *** Test 1 - FO **)
+let test1_pre = (fun () h -> True)
+let test1_post = (fun () h (rfd:resexn file_descr) lt -> (forall fd'. ~((EOpenfile "/etc/passwd" fd') `List.memP` lt)) /\ (Inl? rfd ==> is_open (Inl?.v rfd) (rev lt @ h)))
 
-val ex1_c1post : squash (forall h lt. ex1_ct_pre () h /\ enforced_locally ex1_spec_pi h lt ==> (ex1_ct_post () h (Inr Contract_failure) lt))
-let ex1_c1post = 
+type test1_ct = source_arrow unit file_descr test1_pre test1_post
+
+let test1_pi : monitorable_prop = 
+  fun cmd arg h -> 
+    match cmd, arg with 
+    | Openfile, s -> 
+      if s = "/etc/passwd" then false 
+      else true 
+    | _ -> true
+    
+let test1_ct_rc = (fun () h (rfd:resexn file_descr) lt -> Inl? rfd && (is_open (Inl?.v rfd) (rev lt @ h)))
+let test1_ct_rcs : tree pck_rc = 
+  Node (| unit, resexn file_descr, test1_ct_rc |) 
+    Leaf 
+    Leaf
+
+val test1_c1post : c1typ test1_pre test1_post test1_pi 
+let test1_c1post = 
   let rec aux (h:trace) (lt:trace) : Lemma
-    (requires (enforced_locally ex1_spec_pi h lt))
-    (ensures (ex1_ct_post () h (Inr Contract_failure) lt))
+    (requires (enforced_locally test1_pi h lt))
+    (ensures (test1_post () h (Inr Contract_failure) lt))
     (decreases lt) = (
     match lt with
     | [] -> ()
     | e :: tail -> aux (e::h) tail) in
   Classical.forall_intro_2 (Classical.move_requires_2 aux)
 
-val ex1_c2post : squash (forall x h r lt. ex1_ct_pre () h /\ enforced_locally ex1_spec_pi h lt /\ (ex1_ct_rc x h r lt) ==> ex1_ct_post x h r lt)
-let ex1_c2post = ()
+assume val test1_c2post : c2typ test1_pre test1_post test1_pi test1_ct_rc
+
+//let test1_c2post = ()
+
+let test1_ct_importable (fl:erased tflag) : safe_importable (test1_ct fl) test1_pi test1_ct_rcs fl =
+  safe_importable_arrow_pre_post_args_res _ _ test1_c1post test1_c2post #exportable_unit #importable_file_descr
                                                   
-val ex1_stronger_pis : squash (forall h lt. enforced_locally ex1_inst_pi h lt ==> enforced_locally ex1_spec_pi h lt)
-let ex1_stronger_pis = 
+val test1_stronger_pis : stronger_pis test1_pi test1_pi
+let test1_stronger_pis = 
   let rec aux (h:trace) (lt:trace) : Lemma
-    (requires (enforced_locally ex1_inst_pi h lt))
-    (ensures (enforced_locally ex1_spec_pi h lt))
+    (requires (enforced_locally test1_pi h lt))
+    (ensures (enforced_locally test1_pi h lt))
     (decreases lt) = (match lt with
     | [] -> ()
     | e :: tail -> aux (e::h) tail) in 
   Classical.forall_intro_2 (Classical.move_requires_2 aux)
 
-let ex1 : src_interface = {
-  spec_pi = ex1_spec_pi; inst_pi = ex1_inst_pi;
-  inst_pi_stronger_spec_pi = ex1_stronger_pis;
+[@@ (postprocess_with (fun () -> norm [delta_only [`%test1_ct; `%source_arrow; `%test1_ct_importable]]; trefl ()))]
+let test1 : src_interface = {
+  spec_pi = test1_pi; inst_pi = test1_pi;
+  inst_pi_stronger_spec_pi = test1_stronger_pis;
 
-  ct = (fun fl -> unit -> IIO (resexn file_descr) fl (ex1_ct_pre ()) (ex1_ct_post ()));
-  ct_rcs = Node (| unit, resexn file_descr, ex1_ct_rc |) Leaf Leaf;
+  ct = test1_ct;
+  ct_rcs = test1_ct_rcs;
 
-  ct_importable = (fun fl -> 
-    safe_importable_arrow_pre_post_args_res _ _ ex1_c1post ex1_c2post #exportable_unit #importable_file_descr);
+  ct_importable = test1_ct_importable;
   p_post = (fun _ _ _ lt -> (forall fd'. ~((EOpenfile "/etc/passwd" fd') `List.memP` lt)));
 }
 
-val ex1_prog : prog_src ex1
-let ex1_prog #fl ctx args : IIO int (fl + IOActions) (fun _ -> True) (ex1.p_post args) =
+val test1_prog : prog_src test1
+let test1_prog #fl ctx args : IIO int (fl + IOActions) (fun _ -> True) (test1.p_post args) =
   //let test = static_cmd Openfile "/etc/passwd" in
   let _ = ctx () in
   0 
 
-val ex1_ctx : ctx_src ex1
-let ex1_ctx #fl io_acts eff_rcs () : IIO (resexn file_descr) fl (fun _ -> True) (ex1_ct_post ()) = 
+val test1_ctx : ctx_src test1
+let test1_ctx #fl io_acts eff_rcs () : IIO (resexn file_descr) fl (fun _ -> True) (test1_post ()) = 
   io_acts Openfile "/etc/passwd"
 
-val ex1_ctx_t : ctx_tgt (comp_int_src_tgt ex1)
-let ex1_ctx_t #fl io_acts () : IIOpi (resexn file_descr) fl (comp_int_src_tgt ex1).spec_pi = 
+val test1_ctx_t : ctx_tgt (comp_int_src_tgt test1)
+let test1_ctx_t #fl io_acts () : IIOpi (resexn file_descr) fl (comp_int_src_tgt test1).spec_pi = 
   io_acts Openfile "/etc/passwd"
 
-(** ** Example 2 - HO left 1 **)
-let ex2_pi : monitorable_prop = (fun _ _ _ -> true)
-val ex2_stronger_pis : squash (forall h lt. enforced_locally ex2_pi h lt ==> enforced_locally ex2_pi h lt)
-let ex2_stronger_pis = ()
+(** ** Test 2 - HO left 1 **)
+let test2_pi : monitorable_prop = (fun _ _ _ -> true)
+val test2_stronger_pis : squash (forall h lt. enforced_locally test2_pi h lt ==> enforced_locally test2_pi h lt)
+let test2_stronger_pis = ()
 
-let ex2_cb (fl:erased tflag) = (fd:file_descr -> IIO (resexn unit) fl (fun h -> is_open fd h) (fun _ _ lt -> lt == []))
-let ex2_post = (fun _ h (rfd:resexn file_descr) lt -> Inl? rfd ==> is_open (Inl?.v rfd) (rev lt @ h))
-let ex2_ct (fl:erased tflag) = (cb:ex2_cb fl) -> IIO (resexn file_descr) fl (fun _ -> True) (ex2_post cb)
+let test2_cb (fl:erased tflag) = (fd:file_descr -> IIO (resexn unit) fl (fun h -> is_open fd h) (fun _ _ lt -> lt == []))
+let test2_post = (fun _ h (rfd:resexn file_descr) lt -> Inl? rfd ==> is_open (Inl?.v rfd) (rev lt @ h))
+let test2_ct (fl:erased tflag) = (cb:test2_cb fl) -> IIO (resexn file_descr) fl (fun _ -> True) (test2_post cb)
 
-let ex2_rcs : tree pck_rc =  
+let test2_rcs : tree pck_rc =  
   Node (| unit, resexn file_descr, (fun () h (rfd:resexn file_descr) lt -> Inl? rfd && (is_open (Inl?.v rfd) (rev lt @ h))) |) 
      (Node (| file_descr, unit, (fun fd h _ _ -> is_open fd h) |) Leaf Leaf)
      Leaf
   
-assume val ex2_c1post : #a:Type -> squash (forall (x:a) h lt. enforced_locally ex2_pi h lt ==> (exists r. ex2_post x h r lt))
+assume val test2_c1post : #a:Type -> squash (forall (x:a) h lt. enforced_locally test2_pi h lt ==> (exists r. test2_post x h r lt))
 
-val ex2_c2post : #a:Type -> squash (forall (x:a) h r lt. enforced_locally ex2_pi h lt /\ ((Mkdtuple3?._3 (root ex2_rcs)) () h r lt) ==> ex2_post x h r lt)
-let ex2_c2post #a = ()
+val test2_c2post : #a:Type -> squash (forall (x:a) h r lt. enforced_locally test2_pi h lt /\ ((Mkdtuple3?._3 (root test2_rcs)) () h r lt) ==> test2_post x h r lt)
+let test2_c2post #a = ()
 
-let ex2_ct_importable (fl:erased tflag) : safe_importable (ex2_ct fl) ex2_pi ex2_rcs fl = 
-  let exportable_cb = exportable_arrow_pre_post_args file_descr unit #ex2_pi #(left ex2_rcs) #fl (fun fd h -> is_open fd h) (fun fd _ _ lt -> lt == []) in
+let test2_ct_importable (fl:erased tflag) : safe_importable (test2_ct fl) test2_pi test2_rcs fl = 
+  let exportable_cb = exportable_arrow_pre_post_args file_descr unit #test2_pi #(left test2_rcs) #fl (fun fd h -> is_open fd h) (fun fd _ _ lt -> lt == []) in
   safe_importable_arrow_pre_post_res
     (fun _ _ -> True)  (** pre **)
-    ex2_post       (** post **)
-    (ex2_c1post #(ex2_cb fl))
-    (ex2_c2post #(ex2_cb fl))
+    test2_post       (** post **)
+    (test2_c1post #(test2_cb fl))
+    (test2_c2post #(test2_cb fl))
     #exportable_cb
     #importable_file_descr
 
-[@@ (postprocess_with (fun () -> norm [delta_only [`%ex2_ct; `%ex2_cb;`%ex2_ct_importable]]; trefl ()))]
-let ex2 : src_interface = {
-  spec_pi = ex2_pi; inst_pi = ex2_pi; inst_pi_stronger_spec_pi = ex2_stronger_pis;
-  ct = ex2_ct; ct_rcs = ex2_rcs; ct_importable = ex2_ct_importable; 
+[@@ (postprocess_with (fun () -> norm [delta_only [`%test2_ct; `%test2_cb;`%test2_ct_importable]]; trefl ()))]
+let test2 : src_interface = {
+  spec_pi = test2_pi; inst_pi = test2_pi; inst_pi_stronger_spec_pi = test2_stronger_pis;
+  ct = test2_ct; ct_rcs = test2_rcs; ct_importable = test2_ct_importable; 
   p_post = (fun _ _ _ _ -> True);
 }
 
-val ex2_prog : prog_src ex2
-let ex2_prog #fl ctx args =
+val test2_prog : prog_src test2
+let test2_prog #fl ctx args =
   let _ = ctx (fun fd -> Inl ()) in
   (** return exit code **) 0
 
-val ex2_ctx : ctx_src ex2 
-let ex2_ctx #fl io_acts eff_rcs cb : IIO (resexn file_descr) fl (fun _ -> True) (fun h rfd lt -> Inl? rfd ==> is_open (Inl?.v rfd) (rev lt @ h)) = 
+val test2_ctx : ctx_src test2 
+let test2_ctx #fl io_acts eff_rcs cb : IIO (resexn file_descr) fl (fun _ -> True) (fun h rfd lt -> Inl? rfd ==> is_open (Inl?.v rfd) (rev lt @ h)) = 
   let post1 = root eff_rcs in
   let (| _, pre1 |) = root (left eff_rcs) in 
   let rfd = io_acts Openfile "/etc/passwd" in
@@ -136,8 +166,8 @@ let ex2_ctx #fl io_acts eff_rcs cb : IIO (resexn file_descr) fl (fun _ -> True) 
   | Inl fd -> let _ = pre1 fd in rfd
   | _ -> rfd
 
-val ex2_ctx_t : ctx_tgt (comp_int_src_tgt ex2)
-let ex2_ctx_t #fl io_acts cb : IIOpi (resexn file_descr) fl (comp_int_src_tgt ex2).spec_pi = 
+val test2_ctx_t : ctx_tgt (comp_int_src_tgt test2)
+let test2_ctx_t #fl io_acts cb : IIOpi (resexn file_descr) fl (comp_int_src_tgt test2).spec_pi = 
   let rfd = io_acts Openfile "/etc/passwd" in
   match rfd with
   | Inl fd -> begin
@@ -147,25 +177,25 @@ let ex2_ctx_t #fl io_acts cb : IIOpi (resexn file_descr) fl (comp_int_src_tgt ex
   end
   | _ -> rfd
 
-(** ** Example 3 - HO right 1 **)
-let ex3_pi : monitorable_prop = (fun _ _ _ -> true)
-val ex3_stronger_pis : squash (forall h lt. enforced_locally ex3_pi h lt ==> enforced_locally ex3_pi h lt)
-let ex3_stronger_pis = ()
+(** ** Test 3 - HO right 1 **)
+let test3_pi : monitorable_prop = (fun _ _ _ -> true)
+val test3_stronger_pis : squash (forall h lt. enforced_locally test3_pi h lt ==> enforced_locally test3_pi h lt)
+let test3_stronger_pis = ()
 
-let ex3_cb (fl:erased tflag) = (fd:file_descr -> IIO (resexn unit) fl (fun h -> True) (fun _ _ lt -> True))
-let ex3_post #a = (fun (x:file_descr) h (r:a) lt -> True)
-let ex3_ct (fl:erased tflag) = x:file_descr -> IIO (resexn (ex3_cb fl)) fl (fun _ -> True) (ex3_post x)
+let test3_cb (fl:erased tflag) = (fd:file_descr -> IIO (resexn unit) fl (fun h -> True) (fun _ _ lt -> True))
+let test3_post #a = (fun (x:file_descr) h (r:a) lt -> True)
+let test3_ct (fl:erased tflag) = x:file_descr -> IIO (resexn (test3_cb fl)) fl (fun _ -> True) (test3_post x)
 
-let ex3_rcs : tree pck_rc =  
+let test3_rcs : tree pck_rc =  
   Node (| file_descr, unit, (fun x h r lt -> true) |) 
      Leaf
      (Node (| file_descr, resexn unit, (fun fd h _ _ -> true) |) Leaf Leaf)
 
-let ex3_cb_importable (fl:erased tflag) : safe_importable (ex3_cb fl) ex3_pi (right ex3_rcs) fl = 
+let test3_cb_importable (fl:erased tflag) : safe_importable (test3_cb fl) test3_pi (right test3_rcs) fl = 
   safe_importable_arrow_pre_post_args_res
     #file_descr #unit
-    #ex3_pi
-    #(right ex3_rcs)
+    #test3_pi
+    #(right test3_rcs)
     #fl
     (fun fd h -> True)
     (fun fd _ _ lt -> True)
@@ -174,30 +204,30 @@ let ex3_cb_importable (fl:erased tflag) : safe_importable (ex3_cb fl) ex3_pi (ri
     #exportable_file_descr
     #importable_unit
   
-assume val ex3_c1post : #a:Type -> squash (forall x h lt. enforced_locally ex3_pi h lt ==> (exists (r:a). ex3_post x h r lt))
-//let ex3_c1post #a = () 
-val ex3_c2post : #a:Type -> squash (forall x h (r:a) lt. enforced_locally ex3_pi h lt /\ ((Mkdtuple3?._3 (root ex3_rcs)) x h () lt) ==> ex3_post x h r lt)
-let ex3_c2post #a = ()
+assume val test3_c1post : #a:Type -> squash (forall x h lt. enforced_locally test3_pi h lt ==> (exists (r:a). test3_post x h r lt))
+//let test3_c1post #a = () 
+val test3_c2post : #a:Type -> squash (forall x h (r:a) lt. enforced_locally test3_pi h lt /\ ((Mkdtuple3?._3 (root test3_rcs)) x h () lt) ==> test3_post x h r lt)
+let test3_c2post #a = ()
 
-let ex3_ct_importable (fl:erased tflag) : safe_importable (ex3_ct fl) ex3_pi ex3_rcs fl = 
+let test3_ct_importable (fl:erased tflag) : safe_importable (test3_ct fl) test3_pi test3_rcs fl = 
   safe_importable_arrow_pre_post_args
-    #file_descr #(ex3_cb fl) #ex3_pi #ex3_rcs #fl
+    #file_descr #(test3_cb fl) #test3_pi #test3_rcs #fl
     (fun _ _ -> True)  (** pre **)
-    ex3_post       (** post **)
-    (ex3_c1post #(ex3_cb fl))
-    (ex3_c2post #(ex3_cb fl))
+    test3_post       (** post **)
+    (test3_c1post #(test3_cb fl))
+    (test3_c2post #(test3_cb fl))
     #exportable_file_descr
-    #(safe_importable_is_importable (ex3_cb_importable fl))
+    #(safe_importable_is_importable (test3_cb_importable fl))
 
-[@@ (postprocess_with (fun () -> norm [delta_only [`%ex3_ct; `%ex3_cb;`%ex3_ct_importable;`%ex3_cb_importable;`%safe_importable_is_importable]]; trefl ()))]
-let ex3 : src_interface = {
-  spec_pi = ex3_pi; inst_pi = ex3_pi; inst_pi_stronger_spec_pi = ex3_stronger_pis;
-  ct = ex3_ct; ct_rcs = ex3_rcs; ct_importable = ex3_ct_importable; 
+[@@ (postprocess_with (fun () -> norm [delta_only [`%test3_ct; `%test3_cb;`%test3_ct_importable]]; trefl ()))]
+let test3 : src_interface = {
+  spec_pi = test3_pi; inst_pi = test3_pi; inst_pi_stronger_spec_pi = test3_stronger_pis;
+  ct = test3_ct; ct_rcs = test3_rcs; ct_importable = test3_ct_importable; 
   p_post = (fun _ _ _ _ -> True);
 }
 
-val ex3_prog : prog_src ex3
-let ex3_prog #fl ctx args : IIO int (IOActions + fl) (fun _ -> True) (fun _ _ _ -> True) =
+val test3_prog : prog_src test3
+let test3_prog #fl ctx args : IIO int (IOActions + fl) (fun _ -> True) (fun _ _ _ -> True) =
   match static_cmd Openfile "test.txt" with
   | Inl fd -> begin
     match ctx fd with
@@ -206,10 +236,10 @@ let ex3_prog #fl ctx args : IIO int (IOActions + fl) (fun _ -> True) (fun _ _ _ 
     end
   | Inr err -> -1
 
-val ex3_ctx : ctx_src ex3 
-let ex3_ctx #fl io_acts eff_rcs fd = 
+val test3_ctx : ctx_src test3 
+let test3_ctx #fl io_acts eff_rcs fd = 
   Inl (fun (fd:file_descr) -> Inl ())
 
-val ex3_ctx_t : ctx_tgt (comp_int_src_tgt ex3)
-let ex3_ctx_t #fl io_acts fd : IIOpi (resexn (file_descr -> IIOpi (resexn unit) fl ex3_pi)) fl ex3_pi = 
+val test3_ctx_t : ctx_tgt (comp_int_src_tgt test3)
+let test3_ctx_t #fl io_acts fd : IIOpi (resexn (file_descr -> IIOpi (resexn unit) fl test3_pi)) fl test3_pi = 
   Inl (fun (fd:file_descr) -> Inl ())
